fixup ssaenv, types

MLIR/AST.lean
@@ -81,119 +81,120 @@ inductive Signedness :=
 | Signed   -- si*
 deriving DecidableEq
 
-inductive MLIRType (τ: Code code) :=
-| int: Signedness -> Nat -> MLIRType τ
-| float: Nat -> MLIRType τ
-| tensor1d: MLIRType τ -- tensor of int values.
-| tensor2d: MLIRType τ -- tensor of int values.
-| tensor4d: MLIRType τ -- tensor of int values.
-| index:  MLIRType τ
-| undefined: String → MLIRType τ
-| extended: code → MLIRType τ
-| erased: MLIRType τ -- A type that is erased by dialect retraction.
+-- TODO: make this depend only on `code`
+inductive MLIRType (ty: Type) :=
+| int: Signedness -> Nat -> MLIRType ty
+| float: Nat -> MLIRType ty
+| tensor1d: MLIRType ty -- tensor of int values.
+| tensor2d: MLIRType ty -- tensor of int values.
+| tensor4d: MLIRType ty -- tensor of int values.
+| index:  MLIRType ty
+| undefined: String → MLIRType ty
+| extended: ty → MLIRType ty
+| erased: MLIRType ty -- A type that is erased by dialect retraction.
 
 -- We define "MLIRTy" to be just the basic types outside of any dialect
-abbrev MLIRTy := @MLIRType _ EmptyCode
+abbrev MLIRTy := @MLIRType Void
 -- Other useful abbreviations
-abbrev MLIRType.i1: MLIRType τ := MLIRType.int .Signless 1
-abbrev MLIRType.i32: MLIRType τ := MLIRType.int .Signless 32
+abbrev MLIRType.i1: MLIRType ty := MLIRType.int .Signless 1
+abbrev MLIRType.i32: MLIRType ty := MLIRType.int .Signless 32
 
 -- An SSA value with a type
-abbrev TypedSSAVal (τ: Code code) := SSAVal × MLIRType τ
+abbrev TypedSSAVal (ty: Type) := SSAVal × MLIRType ty
 
 mutual
 
 -- | TODO: factor Symbol out from AttrValue
-inductive AttrValue (α: Code code) :=
-| symbol: String -> AttrValue α -- symbol ref attr
-| str : String -> AttrValue α
-| int : Int -> AttrValue α
-| nat: Nat -> AttrValue α
-| bool : Bool -> AttrValue α
-| float : Float -> AttrValue α
-| affine: AffineMap -> AttrValue α
-| permutation: List Nat -> AttrValue α -- a permutation
-| list: List (AttrValue α) -> AttrValue α
--- | guaranteee: both components will be AttrValue α.Symbol.
+inductive AttrValue (attr: Type) :=
+| symbol: String -> AttrValue attr -- symbol ref attr
+| str : String -> AttrValue attr
+| int : Int -> AttrValue attr
+| nat: Nat -> AttrValue attr
+| bool : Bool -> AttrValue attr
+| float : Float -> AttrValue attr
+| affine: AffineMap -> AttrValue attr
+| permutation: List Nat -> AttrValue attr -- a permutation
+| list: List (AttrValue attr) -> AttrValue attr
+-- | guaranteee: both components will be AttrValue attr.Symbol.
 -- | TODO: factor symbols out.
-| nestedsymbol: AttrValue α -> AttrValue α -> AttrValue α
-| alias: String -> AttrValue α
-| dict: AttrDict α -> AttrValue α
-| opaque_: (dialect: String) -> (value: String) -> AttrValue α
-| opaqueElements: (dialect: String) -> (value: String) -> (type: MLIRType α) -> AttrValue α
-| unit: AttrValue α
-| extended: code → AttrValue α
-| erased: AttrValue α
+| nestedsymbol: AttrValue attr -> AttrValue attr -> AttrValue attr
+| alias: String -> AttrValue attr
+| dict: AttrDict attr -> AttrValue attr
+| opaque_: (dialect: String) -> (value: String) -> AttrValue attr
+| opaqueElements: (dialect: String) -> (value: String) -> (type: MLIRType attr) -> AttrValue attr
+| unit: AttrValue attr
+| extended: attr → AttrValue attr
+| erased: AttrValue attr
 
 -- https://mlir.llvm.org/docs/LangRef/#attributes
 -- | TODO: add support for mutually inductive records / structures
-inductive AttrEntry (α: Code code) :=
+inductive AttrEntry (attr: Type) :=
   | mk: (key: String)
-      -> (value: AttrValue α)
-      -> AttrEntry α
-
-inductive AttrDict (α: Code code) :=
-| mk: List (AttrEntry α) -> AttrDict α
+      -> (value: AttrValue attr)
+      -> AttrEntry attr
+-- TODO: make this depend only on `attr`.
+inductive AttrDict (attr: Type) :=
+| mk: List (AttrEntry attr) -> AttrDict attr
 
 end
 
 -- We define "AttrVal" to be just the basic attributes outside of any dialect
-abbrev AttrVal := @AttrValue _ EmptyCode
+abbrev AttrVal := @AttrValue Void
 
 
 mutual
 -- | TODO: make this `record` when mutual records are allowed?
 -- | TODO: make these arguments optional?
-inductive Op  (α: Code attr) (τ: Code type)where
+-- TODO: make this depend only on `attr`, `type`.
+inductive Op  (attr: Type) (ty: Type) where
  | mk: (name: String)
-      -> (res: List (TypedSSAVal τ))
-      -> (args: List (TypedSSAVal τ))
-      -> (regions: List (Region α τ))
-      -> (attrs: AttrDict α)
-      -> Op α τ
+      -> (res: List (TypedSSAVal ty))
+      -> (args: List (TypedSSAVal ty))
+      -> (regions: List (Region attr ty))
+      -> (attrs: AttrDict attr)
+      -> Op attr ty
 
-inductive Region (α: Code attr) (τ: Code type) where
+inductive Region (attr: Type) (ty: Type) where
 | mk: (name: String)
-      -> (args: List (TypedSSAVal τ))
-      -> (ops: List (Op α τ)) -> Region α τ
+      -> (args: List (TypedSSAVal ty))
+      -> (ops: List (Op attr ty)) -> Region attr ty
 end
 
 -- Attribute definition on the form #<name> = <val>
-inductive AttrDefn (α: Code attr) where
-| mk: (name: String) -> (val: AttrValue α) -> AttrDefn α
+inductive AttrDefn (attr: Type) where
+| mk: (name: String) -> (val: AttrValue attr) -> AttrDefn attr
 
--- | TODO: this seems like a weird exception. Is this really true?
-inductive Module (τ: Code type) (α: Code attr) where
-| mk: (functions: List (Op τ α))
-      -> (attrs: List (AttrDefn α))
-      ->  Module τ α
+inductive Module (ty: Type) (attr: Type) where
+| mk: (functions: List (Op ty attr))
+      -> (attrs: List (AttrDefn attr))
+      ->  Module ty attr
 
 
-def Op.name: Op α τ -> String
+def Op.name: Op attr ty -> String
 | Op.mk name .. => name
 
-def Op.res: Op α τ -> List (TypedSSAVal τ)
+def Op.res: Op attr ty -> List (TypedSSAVal ty)
 | Op.mk _ res .. => res
 
-def Op.resNames: Op α τ → List SSAVal
+def Op.resNames: Op attr ty → List SSAVal
 | Op.mk _ res .. => res.map Prod.fst
 
-def Op.resTypes: Op α τ → List (MLIRType τ)
+def Op.resTypes: Op attr ty → List (MLIRType ty)
 | Op.mk _ res .. => res.map Prod.snd
 
-def Op.args: Op α τ -> List (TypedSSAVal τ)
+def Op.args: Op attr ty -> List (TypedSSAVal ty)
 | Op.mk _ _ args .. => args
 
-def Op.argNames: Op α τ → List SSAVal
+def Op.argNames: Op attr ty → List SSAVal
 | Op.mk _ _ args .. => args.map Prod.fst
 
-def Op.argTypes: Op α τ → List (MLIRType τ)
+def Op.argTypes: Op attr ty → List (MLIRType ty)
 | Op.mk _ _ args .. => args.map Prod.snd
 
-def Op.regions: Op α τ -> List (Region α τ)
+def Op.regions: Op attr ty -> List (Region attr ty)
 | Op.mk _ _ _ regions _ => regions
 
-def Op.attrs: Op α τ -> AttrDict α
+def Op.attrs: Op attr ty -> AttrDict attr
 | Op.mk _ _ _ _ attrs => attrs
 
 
@@ -227,23 +228,23 @@ instance : Coe (List (AttrEntry δ)) (AttrDict δ) where
   coe (v: AttrDict δ) := match v with | AttrDict.mk as => as
 
 
-def Region.name (region: Region α τ): BBName :=
+def Region.name (region: Region attr ty): BBName :=
   match region with
   | Region.mk name args ops => BBName.mk name
 
-def Region.ops (region: Region α τ): List (Op α τ) :=
+def Region.ops (region: Region attr ty): List (Op attr ty) :=
   match region with
   | Region.mk name args ops => ops
 
 
 -- Coercions across dialects
 /-
-variable [δ₁: Dialect α₁ σ₁ ε₁] [δ₂: Dialect α₂ σ₂ ε₂] [c: CoeDialect δ₁ δ₂]
+variable [δ₁: Dialect attr₁ σ₁ ε₁] [δ₂: Dialect attr₂ σ₂ ε₂] [c: CoeDialect δ₁ δ₂]
 -/
 
 /-
-def coeMLIRType [τ: Code ty] [τ': Code ty'] [inj: InjectCode τ τ']:
- MLIRType τ  → MLIRType τ'
+def coeMLIRType [ty: Code ty] [ty': Code ty'] [inj: InjectCode ty ty']:
+ MLIRType ty  → MLIRType ty'
   | .int sgn n   => .int sgn n
   | .float n     => .float n
   | .index       => .index
@@ -252,15 +253,15 @@ def coeMLIRType [τ: Code ty] [τ': Code ty'] [inj: InjectCode τ τ']:
   | .tensor2d => .tensor2d
   | .tensor4d => .tensor4d
   | .erased => .erased
-  | .extended s  => .extended (inj.injectCode τ τ' s)
+  | .extended s  => .extended (inj.injectCode ty ty' s)
 
 
-instance {τ: Code ty} {τ': Code ty'} [inj: InjectCode τ τ']:
-    Coe (MLIRType τ) (MLIRType τ') where
+instance {ty: Code ty} {ty': Code ty'} [inj: InjectCode ty ty']:
+    Coe (MLIRType ty) (MLIRType ty') where
   coe := coeMLIRType
 
 mutual
-variable [δ₁: Dialect α₁ σ₁ ε₁] [δ₂: Dialect α₂ σ₂ ε₂] [c: CoeDialect δ₁ δ₂]
+variable [δ₁: Dialect attr₁ σ₁ ε₁] [δ₂: Dialect attr₂ σ₂ ε₂] [c: CoeDialect δ₁ δ₂]
 
 private def coeAttrValue: AttrValue δ₁ → AttrValue δ₂
   | .nat n => .nat n
@@ -276,9 +277,9 @@ private def coeAttrValue: AttrValue δ₁ → AttrValue δ₂
   | .alias s => .alias s
   | .dict d => .dict (coeAttrDict d)
   | .opaque_ d v => .opaque_ d v
-  | .opaqueElements d v τ => .opaqueElements d v τ
+  | .opaqueElements d v ty => .opaqueElements d v ty
   | .unit => .unit
-  | .extended a => .extended (c.coe_α _ _ a)
+  | .extended a => .extended (c.coe_attr _ _ a)
   | .erased => .erased
 
 private def coeAttrValueList: List (AttrValue δ₁) → List (AttrValue δ₂)
@@ -296,20 +297,20 @@ private def coeAttrDict: AttrDict δ₁ → AttrDict δ₂
   | .mk entries => .mk <| coeAttrEntryList entries
 end
 
-instance {δ₁: Dialect α₁ σ₁ ε₁} {δ₂: Dialect α₂ σ₂ ε₂} [CoeDialect δ₁ δ₂]:
+instance {δ₁: Dialect attr₁ σ₁ ε₁} {δ₂: Dialect attr₂ σ₂ ε₂} [CoeDialect δ₁ δ₂]:
     Coe (AttrValue δ₁) (AttrValue δ₂) where
   coe := coeAttrValue
 
-instance {δ₁: Dialect α₁ σ₁ ε₁} {δ₂: Dialect α₂ σ₂ ε₂} [CoeDialect δ₁ δ₂]:
+instance {δ₁: Dialect attr₁ σ₁ ε₁} {δ₂: Dialect attr₂ σ₂ ε₂} [CoeDialect δ₁ δ₂]:
     Coe (AttrEntry δ₁) (AttrEntry δ₂) where
   coe := coeAttrEntry
 
-instance {δ₁: Dialect α₁ σ₁ ε₁} {δ₂: Dialect α₂ σ₂ ε₂} [CoeDialect δ₁ δ₂]:
+instance {δ₁: Dialect attr₁ σ₁ ε₁} {δ₂: Dialect attr₂ σ₂ ε₂} [CoeDialect δ₁ δ₂]:
     Coe (AttrDict δ₁) (AttrDict δ₂) where
   coe := coeAttrDict
 
 mutual
-variable [δ₁: Dialect α₁ σ₁ ε₁] [δ₂: Dialect α₂ σ₂ ε₂] [c: CoeDialect δ₁ δ₂]
+variable [δ₁: Dialect attr₁ σ₁ ε₁] [δ₂: Dialect attr₂ σ₂ ε₂] [c: CoeDialect δ₁ δ₂]
 
 def coeOp: Op δ₁ → Op δ₂
   | .mk name res args  regions attrs =>
@@ -329,27 +330,27 @@ def coeRegionList: List (Region δ₁) → List (Region δ₂)
 
 end
 
-instance {δ₁: Dialect α₁ σ₁ ε₁} {δ₂: Dialect α₂ σ₂ ε₂} [CoeDialect δ₁ δ₂]:
+instance {δ₁: Dialect attr₁ σ₁ ε₁} {δ₂: Dialect attr₂ σ₂ ε₂} [CoeDialect δ₁ δ₂]:
     Coe (Op δ₁) (Op δ₂) where
   coe := coeOp
 
-instance {δ₁: Dialect α₁ σ₁ ε₁} {δ₂: Dialect α₂ σ₂ ε₂} [CoeDialect δ₁ δ₂]:
+instance {δ₁: Dialect attr₁ σ₁ ε₁} {δ₂: Dialect attr₂ σ₂ ε₂} [CoeDialect δ₁ δ₂]:
     Coe (List (Op δ₁)) (List (Op δ₂)) where
   coe := coeOpList
 
-instance {δ₁: Dialect α₁ σ₁ ε₁} {δ₂: Dialect α₂ σ₂ ε₂} [CoeDialect δ₁ δ₂]:
+instance {δ₁: Dialect attr₁ σ₁ ε₁} {δ₂: Dialect attr₂ σ₂ ε₂} [CoeDialect δ₁ δ₂]:
     Coe (Region δ₁) (Region δ₂) where
   coe := coeRegion
 
-instance {δ₁: Dialect α₁ σ₁ ε₁} {δ₂: Dialect α₂ σ₂ ε₂} [CoeDialect δ₁ δ₂]:
+instance {δ₁: Dialect attr₁ σ₁ ε₁} {δ₂: Dialect attr₂ σ₂ ε₂} [CoeDialect δ₁ δ₂]:
     Coe (List (Region δ₁)) (List (Region δ₂)) where
   coe := coeRegionList
 
-instance {δ₁: Dialect α₁ σ₁ ε₁} {δ₂: Dialect α₂ σ₂ ε₂} [CoeDialect δ₁ δ₂]:
+instance {δ₁: Dialect attr₁ σ₁ ε₁} {δ₂: Dialect attr₂ σ₂ ε₂} [CoeDialect δ₁ δ₂]:
     Coe (Region δ₁) (Region δ₂) where
   coe := coeRegion
 
-instance {δ₁: Dialect α₁ σ₁ ε₁} {δ₂: Dialect α₂ σ₂ ε₂} [CoeDialect δ₁ δ₂]:
+instance {δ₁: Dialect attr₁ σ₁ ε₁} {δ₂: Dialect attr₂ σ₂ ε₂} [CoeDialect δ₁ δ₂]:
     Coe (List (Region δ₁)) (List (Region δ₂)) where
   coe := coeRegionList
 -/
@@ -381,9 +382,9 @@ partial instance : Pretty TensorElem where
 
 -- | TODO: allow typeclass instances inside mutual blocks
 section
-variable {ty} [τ: Code ty]
+variable {ty: Type} [ct: Code ty]
 
-partial def docMLIRType: MLIRType τ → Doc
+partial def docMLIRType: MLIRType ty → Doc
   | .int .Signless k => [doc| "i"k]
   | .int .Unsigned k => [doc| "u"k]
   | .int .Signed k => [doc| "si"k]
@@ -394,11 +395,11 @@ partial def docMLIRType: MLIRType τ → Doc
   | .index => [doc| "index"]
   | .undefined name => [doc| "!" name]
   | .erased => [doc| "erased"]
-  | .extended sig =>  τ.showCode sig
+  | .extended sig =>  ct.showCode sig
 end
 
 mutual
-partial def docAttrVal: AttrValue α → Doc
+partial def docAttrVal [ca: Code attr]: AttrValue attr → Doc
   | .symbol s => "@" ++ doc_surround_dbl_quot s
   | .permutation ps => [doc| "[permutation " (ps),* "]"]
   | .nestedsymbol s t => (docAttrVal s) ++ "::" ++ (docAttrVal t)
@@ -414,33 +415,33 @@ partial def docAttrVal: AttrValue α → Doc
   | .opaque_ dialect val => [doc| "#" (dialect) "<"  (val) ">"]
   | .opaqueElements dialect val ty => [doc| "#opaque<" (dialect) ","  (val) ">" ":" (docMLIRType ty)]
   | .unit => "()"
-  | .extended a => α.showCode a
+  | .extended a => ca.showCode a
   | .erased => "<erased>"
 
-partial def docAttrEntry: AttrEntry α → Doc
+partial def docAttrEntry [ca: Code attr]: AttrEntry attr → Doc
   | .mk k v => k ++ " = " ++ (docAttrVal v)
 
-partial def docAttrDict: AttrDict α → Doc
+partial def docAttrDict [ca: Code attr]: AttrDict attr → Doc
   | .mk attrs =>
       if List.isEmpty attrs
       then Doc.Text ""
       else "{" ++ Doc.Nest (vintercalate_doc (attrs.map docAttrEntry)  ", ")  ++ "}"
 end
 
-instance : Pretty (MLIRType τ) where
+instance [Code ty] : Pretty (MLIRType ty) where
  doc := docMLIRType
 
-instance : Pretty (AttrValue α) where
+instance [Code attr] : Pretty (AttrValue attr) where
  doc := docAttrVal
 
-instance : Pretty (AttrEntry α) where
+instance  [Code attr]: Pretty (AttrEntry attr) where
   doc := docAttrEntry
 
-instance : Pretty (AttrDict α) where
+instance [Code attr]: Pretty (AttrDict attr) where
    doc := docAttrDict
 
-instance : Pretty (AttrDefn α) where
-  doc (v: AttrDefn α) :=
+instance [Code attr]: Pretty (AttrDefn attr) where
+  doc (v: AttrDefn attr) :=
   match v with
   | AttrDefn.mk name val => "#" ++ name ++ " := " ++ (doc val)
 
@@ -456,7 +457,7 @@ instance : ToFormat SSAVal where
 -- | would be so much nicer if I could pretend that these had real instances.
 mutual
 
-def op_to_doc (op: Op α τ): Doc :=
+def op_to_doc [Code attr] [Code ty] (op: Op attr ty): Doc :=
     match op with
     | (Op.mk name res args rgns attrs) =>
         /- v3: macros + if stuff-/
@@ -487,12 +488,12 @@ def op_to_doc (op: Op α τ): Doc :=
 
         doc_name ++ doc_args ++  doc_bbs ++ doc_rgns ++ doc attrs ++ " : " ++ doc ty -/
 
-def list_op_to_doc: List (Op α τ) → List Doc
+def list_op_to_doc [Code attr] [Code ty]: List (Op attr ty) → List Doc
   | [] => []
   | op :: ops => op_to_doc op :: list_op_to_doc ops
 
 -- | TODO: fix the dugly syntax
-def rgn_to_doc: Region α τ → Doc
+def rgn_to_doc [Code attr] [Code ty]: Region attr ty → Doc
   | (Region.mk name args ops) =>
     [doc| {
         (ifdoc args.isEmpty
@@ -500,18 +501,18 @@ def rgn_to_doc: Region α τ → Doc
          else  "^" name "(" (args.map $ fun (v, t) => [doc| v ":" t]),* ")" ":");
         (nest list_op_to_doc ops);* ; } ]
 
-def list_rgn_to_doc: List (Region α τ) → List Doc
+def list_rgn_to_doc [Code attr] [Code ty]: List (Region attr ty) → List Doc
   | [] => []
   | r :: rs => rgn_to_doc r :: list_rgn_to_doc rs
 end
 
-instance : Pretty (Op α τ) where
+instance [Code attr] [Code ty]: Pretty (Op attr ty) where
   doc := op_to_doc
 
-instance : Pretty (Region α τ) where
+instance [Code attr] [Code ty]: Pretty (Region attr ty) where
   doc := rgn_to_doc
 
-instance : Pretty (Region α τ) where
+instance [Code attr] [Code ty]: Pretty (Region attr ty) where
   doc := rgn_to_doc
 
 def AttrEntry.key (a: AttrEntry δ): String :=
@@ -523,61 +524,61 @@ match a with
 | AttrEntry.mk k v => v
 
 
-def AttrDict.empty : AttrDict α := AttrDict.mk []
+def AttrDict.empty : AttrDict attr := AttrDict.mk []
 
-def Op.empty (name: String) : Op α τ := Op.mk name [] [] [] AttrDict.empty
+def Op.empty (name: String) : Op attr ty := Op.mk name [] [] [] AttrDict.empty
 
 -- | TODO: needs to happen in a monad to ensure that ty has the right type!
-def Op.addArg (o: Op α τ) (arg: TypedSSAVal τ): Op α τ :=
+def Op.addArg (o: Op attr ty) (arg: TypedSSAVal ty): Op attr ty :=
   match o with
   | Op.mk name res args regions attrs =>
     Op.mk name res (args ++ [arg])  regions attrs
 
-def Op.addResult (o: Op α τ) (new_res: TypedSSAVal τ): Op α τ :=
+def Op.addResult (o: Op attr ty) (new_res: TypedSSAVal ty): Op attr ty :=
  match o with
  | Op.mk name res args  regions attrs =>
     Op.mk name (res ++ [new_res]) args  regions attrs
 
-def Op.appendRegion (o: Op α τ) (r: Region α τ): Op α τ :=
+def Op.appendRegion (o: Op attr ty) (r: Region attr ty): Op attr ty :=
   match o with
   | Op.mk name res args regions attrs =>
       Op.mk name res args (regions ++ [r]) attrs
 
 
 -- | Note: AttrEntry can be given as String × AttrValue
-def AttrDict.add [α: Code attr] (attrs: AttrDict α) (entry: AttrEntry α): AttrDict α :=
+def AttrDict.add [Code attr] (attrs: AttrDict attr) (entry: AttrEntry attr): AttrDict attr :=
     (entry :: attrs)
 
-def AttrDict.find [α: Code attr] (attrs: AttrDict α) (name: String): Option (AttrValue α) :=
+def AttrDict.find [Code attr] (attrs: AttrDict attr) (name: String): Option (AttrValue attr) :=
   match attrs with
   | AttrDict.mk entries =>
       match entries.find? (fun entry => entry.key == name) with
       | some v => v.value
       | none => none
 
-def AttrDict.find_nat (attrs: AttrDict α)
+def AttrDict.find_nat [Code attr] (attrs: AttrDict attr)
   (name: String): Option Nat :=
   match attrs.find name with
   | .some (AttrValue.nat i) =>  .some i
   | _ => .none
 
-def AttrDict.find_int [α: Code attr] (attrs: AttrDict α)
+def AttrDict.find_int [Code attr] (attrs: AttrDict attr)
   (name: String): Option Int :=
   match attrs.find name with
   | .some (AttrValue.int i) => .some i
   | _ => .none
 
-def AttrDict.find_int' [α: Code attr] (attrs: AttrDict α) (name: String): Option Int :=
+def AttrDict.find_int' [Code attr] (attrs: AttrDict attr) (name: String): Option Int :=
   match attrs.find name with
   | .some (AttrValue.int i) =>  .some i
   | _ => .none
 
-@[simp] theorem AttrDict.find_none [α: Code attr]:
-    AttrDict.find (α := α) (AttrDict.mk []) name = none := by
+@[simp] theorem AttrDict.find_none [Code attr]:
+    AttrDict.find (attr := attr) (AttrDict.mk []) name = none := by
   simp [AttrDict.find, List.find?]
 
-@[simp] theorem AttrDict.find_next [α: Code attr] (v: AttrValue α)
-  (l: List (AttrEntry α)):
+@[simp] theorem AttrDict.find_next [Code attr] (v: AttrValue attr)
+  (l: List (AttrEntry attr)):
     AttrDict.find (AttrDict.mk (AttrEntry.mk n v :: l)) n' =
     if n == n' then some v else AttrDict.find (AttrDict.mk l) n' := by
   cases H: n == n' <;>
@@ -587,56 +588,56 @@ def AttrDict.addString (attrs: AttrDict δ) (k: String) (v: String): AttrDict δ
     AttrEntry.mk k (v: AttrValue δ) :: attrs
 
 
-def Op.addAttr (o: Op α τ) (k: String) (v: AttrValue α): Op α τ :=
+def Op.addAttr [Code attr] (o: Op attr ty) (k: String) (v: AttrValue attr): Op attr ty :=
  match o with
  | Op.mk name res args regions attrs =>
     Op.mk name res args regions (attrs.add (k, v))
 
-def Region.empty (name: String): Region α τ := Region.mk name [] []
-def Region.appendOp (bb: Region α τ) (op: Op α τ): Region α τ :=
+def Region.empty (name: String): Region attr ty := Region.mk name [] []
+def Region.appendOp (bb: Region attr ty) (op: Op attr ty): Region attr ty :=
   match bb with
   | Region.mk name args bbs => Region.mk name args (bbs ++ [op])
 
-def Region.appendOps (bb: Region α τ) (ops: List (Op α τ)): Region α τ :=
+def Region.appendOps (bb: Region attr ty) (ops: List (Op attr ty)): Region attr ty :=
   match bb with
   | Region.mk name args bbs => Region.mk name args (bbs ++ ops)
 
 
-instance : Pretty (Op α τ) where
+instance [Code attr] [Code ty]: Pretty (Op attr ty) where
   doc := op_to_doc
 
-instance : Pretty (Region α τ) where
+instance [Code attr] [Code ty]: Pretty (Region attr ty) where
   doc := rgn_to_doc
 
 instance [Pretty a] : ToString a where
   toString (v: a) := layout80col (doc v)
 
-instance : ToFormat (Op α τ) where
-    format (x: Op α τ) := layout80col (doc x)
+instance [Code attr] [Code ty]: ToFormat (Op attr ty) where
+    format (x: Op attr ty) := layout80col (doc x)
 
 
-instance : Inhabited (MLIRType τ) where
+instance : Inhabited (MLIRType ty) where
   default := MLIRType.undefined "INHABITANT"
 
-instance : Inhabited (AttrValue α) where
+instance : Inhabited (AttrValue attr) where
   default := AttrValue.str "INHABITANT"
 
-instance : Inhabited (Op α τ) where
+instance : Inhabited (Op attr ty) where
   default := Op.empty "INHABITANT"
 
-instance : Inhabited (Region α τ) where
+instance : Inhabited (Region attr ty) where
   default := Region.empty "INHABITANT"
 
-instance : Pretty (Module α τ) where
-  doc (m: Module α τ) :=
+instance  [Code attr] [Code ty]: Pretty (Module attr ty) where
+  doc (m: Module attr ty) :=
     match m with
     | Module.mk fs attrs =>
       Doc.VGroup (attrs.map doc ++ fs.map doc)
 
-def Region.fromOps (os: List (Op α τ)) (name: String := "entry"): Region α τ :=
+def Region.fromOps (os: List (Op attr ty)) (name: String := "entry"): Region attr ty :=
   Region.mk name [] os
 
-def Region.setArgs (bb: Region α τ) (args: List (TypedSSAVal τ)) : Region α τ :=
+def Region.setArgs (bb: Region attr ty) (args: List (TypedSSAVal ty)) : Region attr ty :=
 match bb with
   | (Region.mk name _ ops) => (Region.mk name args ops)
 
